Improve pushD

src/ImplicitQueue.v
@@ -10,55 +10,118 @@ Inductive Front (A : Type) : Type :=
 | FOne : A -> Front A
 | FTwo : A -> A -> Front A.
 
+Inductive FrontA (A : Type) : Type :=
+| FOneA : T A -> FrontA A
+| FTwoA : T A -> T A -> FrontA A.
+
+#[global]
+Instance Exact_Front (A : Type) : Exact (Front A) (FrontA A) :=
+  fun u => match u with
+           | FOne x => FOneA (Thunk x)
+           | FTwo x y => FTwoA (Thunk x) (Thunk y)
+           end.
+
 Inductive Rear (A : Type) : Type :=
 | RZero : Rear A
 | ROne : A -> Rear A.
 
+Inductive RearA (A : Type) : Type :=
+| RZeroA : RearA A
+| ROneA : T A -> RearA A.
+
+#[global]
+Instance Exact_Rear (A : Type) : Exact (Rear A) (RearA A) :=
+  fun u => match u with
+           | RZero => RZeroA
+           | ROne x => ROneA (Thunk x)
+           end.
+
 Inductive Queue (A : Type) : Type :=
-| Nil  : Queue A
+| Nil : Queue A
 | Deep : Front A -> Queue (A * A) -> Rear A -> Queue A.
+
+Inductive QueueA (A : Type) : Type :=
+| NilA : QueueA A
+| DeepA : T (FrontA A) -> T (QueueA (A * A)) -> T (RearA A) -> QueueA A.
 
 Fixpoint push (A : Type) (q : Queue A) (x : A) : Queue A :=
   match q with
   | Nil => Deep (FOne x) Nil RZero
   | Deep f q RZero => Deep f q (ROne x)
-  | Deep f q (ROne y) => Deep f (push q (x, y)) RZero
+  | Deep f q (ROne y) => Deep f (push q (y, x)) RZero
   end.
+
+Definition pairD (A B : Type) (p : T (A * B)) : T A * T B :=
+  match p with
+  | Undefined => (Undefined, Undefined)
+  | Thunk (x, y) => (Thunk x, Thunk y)
+  end.
+
+Fixpoint pushD (A : Type) (q : Queue A) (x : A) (outD : QueueA A) : Tick (T (QueueA A) * T A) :=
+  Tick.tick >>
+    match q with
+    | Nil => Tick.ret (Thunk NilA, Thunk x)
+    | Deep f q RZero => match outD with
+                        | DeepA fA qA (Thunk (ROneA xA)) => Tick.ret (Thunk (DeepA fA qA (Thunk RZeroA)), xA)
+                        | _ => bottom
+                        end
+    | Deep f q (ROne y) => match outD with
+                           | DeepA fA qA (Thunk RZeroA) => let+ (qD, pD) := thunkD (pushD q (y, x)) qA in
+                                                           let (yD, xD) := pairD pD
+                                                           in Tick.ret (Thunk (DeepA fA qD (Thunk (ROneA yD))), xD)
+                           | _ => bottom
+                           end
+    end.
 
 Fixpoint pop (A : Type) (q : Queue A) : option (A * Queue A) :=
   match q with
   | Nil => None
   | Deep (FTwo x y) q r => Some (x, Deep (FOne y) q r)
-  | Deep (FOne x) q r => Some (x, match pop q with
-                                  | Some ((y, z), q) => Deep (FTwo y z) q r
-                                  | None => match r with
-                                            | RZero => Nil
-                                            | ROne y => Deep (FOne y) Nil RZero
-                                            end
-                                  end)
+  | Deep (FOne x) q r => let q' := match pop q with
+                                   | Some ((y, z), q) => Deep (FTwo y z) q r
+                                   | None => match r with
+                                             | RZero => Nil
+                                             | ROne y => Deep (FOne y) Nil RZero
+                                             end
+                                   end
+                         in Some (x, q')
   end.
 
-Inductive QueueA (A : Type) : Type :=
-| NilA : QueueA A
-| DeepA : Front A -> T (QueueA (A * A)) -> Rear A -> QueueA A.
 
-#[global]
-Instance Exact_Queue : forall (A : Type), Exact (Queue A) (QueueA A) :=
-  fix Exact_Queue _ q := match q with
-                         | Nil => NilA
-                         | Deep f q r => DeepA f (Thunk (Exact_Queue _ q)) r
-                         end.
+(* Fixpoint popD (A : Type) (q : Queue A) (outD : option (T A * T (QueueA A))) : Tick (T (QueueA A)) := *)
+(*   Tick.tick >> *)
+(*     match q with *)
+(*     | Nil => Tick.ret (Thunk NilA) *)
+(*     | Deep (FTwo _ _) _ _ => match outD with *)
+(*                              | Some (xA, Thunk (DeepA (Thunk (FOneA yA)) qA rA)) => *)
+(*                                  Tick.ret (Thunk (DeepA (Thunk (FTwoA xA yA)) qA rA)) *)
+(*                              | _ => Tick.ret bottom *)
+(*                              end *)
+(*     | Deep (FOne _) q _ => match outD with *)
+(*                            | Some (xA, Thunk (DeepA (Thunk (FTwoA yA zA)) qA rA)) => *)
+(*                                      let+ rD := thunkD (popD q) qA in *)
+(*                                      let q' := thunkD (fun r => match r with *)
+(*                                                                 | RZeroA => Nil *)
+(*                                                                 | ROneA _ => Nil *)
+(*                                                                 end) rD *)
+(*                                        (* match rD with *) *)
+(*                                        (*         | Undefined => Tick.ret bottom *) *)
+(*                                        (*         | _ => Tick.ret bottom *) *)
+(*                                        (*         end *) *)
+(*                                      in Tick.ret bottom *)
+(*                            | _ => Tick.ret bottom *)
+(*                            end *)
+(*     end. *)
 
-Fixpoint pushD (A : Type) (q : Queue A) (x : A) (outD : QueueA A) : Tick (T (QueueA A)) :=
-  match q with
-  | Nil => Tick.ret (Thunk (DeepA (FOne x) (Thunk NilA) RZero))
-  | Deep f q RZero => match outD with
-                      | DeepA _ qA _ => Tick.ret (Thunk (DeepA f qA (ROne x)))
-                      | _ => bottom
-                      end
-  | Deep f q (ROne y) => match outD with
-                         | DeepA _ qA _ => let+ qD := thunkD (pushD q (x, y)) qA in
-                                           Tick.ret (Thunk (DeepA f qD RZero))
-                         | _ => bottom
-                         end
-  end.
+
+        (* let+ qD := thunkD (popD q) *)
+    (* end. *)
+
+                         (*               let q' := match pop q with *)
+                         (*           | Some ((y, z), q) => Deep (FTwo y z) q r *)
+                         (*           | None => match r with *)
+                         (*                     | RZero => Nil *)
+                         (*                     | ROne y => Deep (FOne y) Nil RZero *)
+                         (*                     end *)
+                         (*           end *)
+                         (* in Some (x, q') *)
